theories/stdpp_img.v
@@ -1,0 +1,99 @@
+From Coq Require Import ssreflect.
+From stdpp Require Import countable gmap list.
+
+(** The function [img m] should yield the image/codomain of [m]. That is a finite
+set of type [D] that contains the values that appear in [m].
+[D] is an output of the typeclass, i.e., there can be only one instance per map
+type [M]. *)
+Class Img (M D : Type) := img: M → D.
+Global Hint Mode Img ! - : typeclass_instances.
+Global Instance: Params (@img) 3 := {}.
+Global Arguments img : clear implicits.
+Global Arguments img {_ _ _} !_ / : simpl nomatch, assert.
+
+
+Class FinMapImg K A M D
+  `{Img (M A) D, FMap M,
+    ∀ A, Lookup K A (M A), ∀ A, Empty (M A), ∀ A, PartialAlter K A (M A),
+    OMap M, Merge M, ∀ A, FinMapToList K A (M A), EqDecision K,
+    ElemOf A D, Empty D, Singleton A D,
+    Union D, Intersection D, Difference D} := {
+  finmap_dom_map :> FinMap K M;
+  finmap_dom_set :> Set_ A D;
+  elem_of_img (m:M A) (v:A) : v ∈ img m <-> ∃ (k:K), m !! k = Some v
+}.
+
+Section fin_map_img.
+  Context `{FinMapImg K A M D}.
+
+  Lemma img_union:
+    ∀ (m1 m2:M A) (v:A),
+    v ∈ img (m1 ∪ m2) ->
+    v ∈ img m1 \/ v ∈ img m2.
+  Proof.
+    intros m1 m2 v Hv12.
+    (* destruct (elem_of_img (m1 ∪ m2) v) as . *)
+    rewrite (elem_of_img (m1 ∪ m2) v) in Hv12.
+    destruct Hv12 as [k Hv12].
+    destruct (lookup_union_Some_raw m1 m2 k v) as [Hspec _].
+    destruct (Hspec Hv12) as [Hm | [_ Hm]].
+    left. 2: right.
+    all: rewrite elem_of_img; exists k; exact Hm.
+  Qed.
+
+  Lemma img_empty:
+    img (@empty (M A) _) ≡@{D} ∅.
+  Proof.
+    rewrite set_equiv.
+    intros x.
+    split; intros Hempty.
+    apply elem_of_img in Hempty. destruct Hempty as [k Hk].
+    rewrite lookup_empty in Hk. discriminate.
+    rewrite elem_of_empty in Hempty. contradiction Hempty.
+  Qed.
+
+  Lemma img_singleton (k:K) (v:A) : img ({[ k := v ]} : M A) ≡@{D} {[ v ]}.
+  Proof.
+    rewrite set_equiv. intros x.
+    rewrite elem_of_img. rewrite elem_of_singleton.
+    setoid_rewrite lookup_singleton_Some. set_solver.
+  Qed.
+
+  Lemma img_empty_L `{!LeibnizEquiv D}:
+    img (@empty (M A) _) = ∅.
+  Proof. unfold_leibniz. exact img_empty. Qed.
+
+  Lemma img_singleton_L `{!LeibnizEquiv D} (k:K) (v:A) : img ({[ k := v ]} : M A) = {[ v ]}.
+  Proof. unfold_leibniz. apply img_singleton. Qed.
+End fin_map_img.
+
+Global Instance fin_map_img K A M D
+  `{FinMapToList K A M, Singleton A D, Empty D, Union D}
+: Img M D := map_to_set (fun _ a => a).
+Global Instance gmap_img K A
+  `{EqDecision K, Countable K, EqDecision A, Countable A}
+: Img (gmap K A) (gset A) := fin_map_img K A (gmap K A) (gset A).
+
+Lemma elem_of_img_rev {K A M D} `{FinMapImg K A M D} :
+  ∀ (m:M A) (k:K) (v:A), m !! k = Some v -> v ∈ img m.
+Proof.
+  intros m k v Hmkv. rewrite elem_of_img. exists k. exact Hmkv.
+Qed.
+
+Global Instance fin_map_img_spec K A M D
+  `{HFinMap:FinMap K M} `{HFinSet:FinSet A D} : FinMapImg K A M D.
+Proof.
+  split.
+  exact HFinMap.
+  apply fin_set_set.
+  unfold img, fin_map_img.
+  intros m v.
+  rewrite elem_of_map_to_set.
+  split.
+  intros [k [v' [mk_v' v'_v]]]. exists k. rewrite v'_v in mk_v'. exact mk_v'.
+  intros [k mk_v]. exists k. exists v. split. exact mk_v. reflexivity.
+Qed.
+
+Global Instance gmap_imp_spec K A
+ `{EqDecision K, Countable K, EqDecision A, Countable A}
+: FinMapImg K A (gmap K) (gset A) := fin_map_img_spec K A (gmap K) (gset A).
